proofs/semantics/PrismSem.lean
@@ -4,3 +4,5 @@ import PrismSem.Semantics
 import PrismSem.Instrument
 import PrismSem.Encode
 import PrismSem.Memory
+import PrismSem.MemEncode
+import PrismSem.Examples
